\documentclass[12pt]{article}
 
\usepackage[margin=1in]{geometry} 
\usepackage{enumitem}
\usepackage{amsmath}
\usepackage{booktabs}

\newenvironment{blockquote}{%
  \par%
  \medskip
  \leftskip=2em%
  \noindent\ignorespaces}{%
  \par\medskip}

\begin{document}
 
\title{Homework 6}
\author{Jacob Nisnevich \textemdash \hspace{2px} 804375355 \\ \\
CS 161}
 
\maketitle
 
\begin{enumerate}
	\item For each pair of atomic sentences, give the most general unifier if it exists:

		\begin{enumerate}
			\item $P(A, B, B), P(x, y, z)$

			$\sigma = \{x \backslash A, y \backslash B, z \backslash B\}$

			\item $Q(y, G(A, B)), Q(G(x, x), y)$

			Does not exist

			\item $R(x, A, z), R(B, y, z)$

			$\sigma = \{x \backslash B, y \backslash A\}$

			\item $\text{Older}(\text{Father}(y), y), \text{Older}(\text{Father}(x), \text{John})$

			$\sigma = \{x \backslash \text{John}, y \backslash \text{John}\}$

			\item $\text{Knows}(\text{Father}(y), y), \text{Knows}(x, x)$

			Does not exist
		\end{enumerate}

	\item Translate the following sentences into formulas in first-order logic:

		\begin{enumerate}
			\item There exists at most one $x$ such that $P(x)$

			$\forall x \forall y ((P(x) \land P(y)) \Rightarrow x = y)$

			\item There exists exactly one $x$ such that $P(x)$

			$\exists x (P(x) \land \forall y (P(y) \Rightarrow x = y))$

			\item There exists at least two $x$ such that $P(x)$

			$\exists x \exists y (P(x) \land P(y) \land \neg (x = y))$

			\item There exists at most two $x$ such that $P(x)$

			$\forall x \forall y \forall z ((P(x) \land P(y) \land P(z)) \Rightarrow (x = y \lor y = z \lor x = z))$

			\item There exists exactly two $x$ such that $P(x)$

			$\exists x \exists y (P(x) \land P(y) \land x \neq y \land \forall z (P(z) \Rightarrow z = x \lor z = y))$
		\end{enumerate}

	\item For each knowledge base, determine whether it is satisfiable. Justify your answer intuitively.

		\begin{enumerate}
			\item $P(A), (\exists x) (\neg P(x))$

			This knowledge base is satisfiable. It is only known that $P(x)$ returns true for $A$.

			\item $P(A), (\forall x) (\neg P(x))$

			This knowledge base is not satisfiable. As it is given that $P(x)$ is true for $A$, it is impossible for $P(x)$ to always be false.

			\item $(\forall x)(\exists y)(P(x, y)), (\forall x)(\neg P(x, x)))$

			This knowledge base is satisfiable. This is true if $x$ and $y$ are different in $P(x, y)$.

			\item $(\forall x)(P(x) \Rightarrow (\exists x)(P(x)))$

			This knowledge base is satisfiable. This is trivially true as the validity of $P(x)$ for all $x$ implies that there is some $P(x)$.

			\item $(\forall x)(P(x) \Rightarrow (\forall x)(P(x)))$

			This knowledge base is satisfiable. This works in the case that $x$ satisfies $P(x)$ and everyone else satisfies $P(x)$.

		\end{enumerate}

	\item Consider the following sentences:

		\begin{itemize}
			\item John likes all kinds of food.
			\item Apples are food.
			\item Chicken is food.
			\item Anything anyone eats and isn't killed by is food.
			\item If you are killed by something, you are not alive.
			\item Bill eats peanuts and is still alive. *
			\item Sue eats everything Bill eats.
		\end{itemize}

		\begin{enumerate}
			\item Translate these sentences into formulas in first-order logic.

			\begin{itemize}
				\item $\forall x (\text{Food}(x) \Rightarrow \text{Likes}(\text{John}, x))$
				\item $\text{Food}(\text{Apples})$
				\item $\text{Food}(\text{Chicken})$
				\item $\forall x \forall y ((\text{Eats}(x, y) \land \neg \text{\text{Kills}}(y, x)) \Rightarrow \text{Food}(y))$
				\item $\forall x \forall y (\text{Kills}(y, x) \Rightarrow \neg \text{Alive}(x))$
				\item $\text{Eats}(\text{Bill}, \text{Peanuts}) \land \text{Alive}(\text{Bill})$
				\item $\forall x (\text{Eats}(\text{Bill}, x) \Rightarrow \text{Eats}(\text{Sue}, x)$
			\end{itemize}

			\item Convert the formulas of part (a) into CNF (also called clausal form).

			\begin{enumerate}[label=\arabic*.]
				\item Eliminate $\Rightarrow$ and $\Leftrightarrow$
					\begin{itemize}
						\item $\forall x (\neg \text{Food}(x) \lor \text{Likes}(\text{John}, x))$
						\item $\text{Food}(\text{Apples})$
						\item $\text{Food}(\text{Chicken})$
						\item $\forall x \forall y (\neg (\text{Eats}(x, y) \land \neg \text{\text{Kills}}(y, x)) \lor \text{Food}(y))$
						\item $\forall x \forall y (\neg \text{Kills}(y, x) \lor \neg \text{Alive}(x))$
						\item $\text{Eats}(\text{Bill}, \text{Peanuts}) \land \text{Alive}(\text{Bill})$
						\item $\forall x (\neg \text{Eats}(\text{Bill}, x) \lor \text{Eats}(\text{Sue}, x)$
					\end{itemize}
				\item Move $\neg$ inwards
					\begin{itemize}
						\item $\forall x (\neg \text{Food}(x) \lor \text{Likes}(\text{John}, x))$
						\item $\text{Food}(\text{Apples})$
						\item $\text{Food}(\text{Chicken})$
						\item $\forall x \forall y (\neg \text{Eats}(x, y) \lor  \text{\text{Kills}}(y, x) \lor \text{Food}(y))$
						\item $\forall x \forall y (\neg \text{Kills}(y, x) \lor \neg \text{Alive}(x))$
						\item $\text{Eats}(\text{Bill}, \text{Peanuts}) \land \text{Alive}(\text{Bill})$
						\item $\forall x (\neg \text{Eats}(\text{Bill}, x) \lor \text{Eats}(\text{Sue}, x)$
					\end{itemize}
				\item Standardize variables
					\begin{itemize}
						\item $\forall a (\neg \text{Food}(a) \lor \text{Likes}(\text{John}, a))$
						\item $\text{Food}(\text{Apples})$
						\item $\text{Food}(\text{Chicken})$
						\item $\forall b \forall c (\neg \text{Eats}(b, c) \lor  \text{\text{Kills}}(c, b) \lor \text{Food}(c))$
						\item $\forall d \forall e (\neg \text{Kills}(e, d) \lor \neg \text{Alive}(d))$
						\item $\text{Eats}(\text{Bill}, \text{Peanuts}) \land \text{Alive}(\text{Bill})$
						\item $\forall f (\neg \text{Eats}(\text{Bill}, f) \lor \text{Eats}(\text{Sue}, f)$
					\end{itemize}
				\item Skolemization
					\begin{itemize}
						\item $\forall a (\neg \text{Food}(a) \lor \text{Likes}(\text{John}, a))$
						\item $\text{Food}(\text{Apples})$
						\item $\text{Food}(\text{Chicken})$
						\item $\forall b \forall c (\neg \text{Eats}(b, c) \lor  \text{\text{Kills}}(c, b) \lor \text{Food}(c))$
						\item $\forall d \forall e (\neg \text{Kills}(e, d) \lor \neg \text{Alive}(d))$
						\item $\text{Eats}(\text{Bill}, \text{Peanuts}) \land \text{Alive}(\text{Bill})$
						\item $\forall f (\neg \text{Eats}(\text{Bill}, f) \lor \text{Eats}(\text{Sue}, f)$
					\end{itemize}
				\item Get rid of universal quantifiers
					\begin{itemize}
						\item $\neg \text{Food}(a) \lor \text{Likes}(\text{John}, a)$
						\item $\text{Food}(\text{Apples})$
						\item $\text{Food}(\text{Chicken})$
						\item $\neg \text{Eats}(b, c) \lor  \text{\text{Kills}}(c, b) \lor \text{Food}(c)$
						\item $\neg \text{Kills}(e, d) \lor \neg \text{Alive}(d)$
						\item $\text{Eats}(\text{Bill}, \text{Peanuts}) \land \text{Alive}(\text{Bill})$
						\item $\neg \text{Eats}(\text{Bill}, f) \lor \text{Eats}(\text{Sue}, f)$
					\end{itemize}
				\item Distribute $\lor$ and $\land$
					\begin{itemize}
						\item $\neg \text{Food}(a) \lor \text{Likes}(\text{John}, a)$
						\item $\text{Food}(\text{Apples})$
						\item $\text{Food}(\text{Chicken})$
						\item $\neg \text{Eats}(b, c) \lor  \text{\text{Kills}}(c, b) \lor \text{Food}(c)$
						\item $\neg \text{Kills}(e, d) \lor \neg \text{Alive}(d)$
						\item $\text{Eats}(\text{Bill}, \text{Peanuts}) \land \text{Alive}(\text{Bill})$
						\item $\neg \text{Eats}(\text{Bill}, f) \lor \text{Eats}(\text{Sue}, f)$
					\end{itemize}
			\end{enumerate}

			\item Prove that John likes peanuts using resolution.

				\begin{tabular}{ l l r }
					1. & $\neg \text{Food}(a) \lor \text{Likes}(\text{John}, a)$ & \\
					2. & $\text{Food}(\text{Apples})$ & \\
					3. & $\text{Food}(\text{Chicken})$ & \\
					4. & $\neg \text{Eats}(b, c) \lor  \text{\text{Kills}}(c, b) \lor \text{Food}(c)$ & \\
					5. & $\neg \text{Kills}(e, d) \lor \neg \text{Alive}(d)$ & \\
					6. & $\text{Eats}(\text{Bill}, \text{Peanuts})$ & \\
					7. & $\text{Alive}(\text{Bill})$ & \\
					8. & $\neg \text{Eats}(\text{Bill}, f) \lor \text{Eats}(\text{Sue}, f)$ & \\
					9. & $\neg \text{Likes}(\text{John}, \text{Peanuts})$ & \\
					\toprule
					10. & $\neg \text{Food}(\text{Peanuts})$ & 1, 9 \\
					11. & $\neg \text{Kills}(e, \text{Bill})$ & 5, 7 \\
					12. & $\neg \text{Eats}(\text{Bill}, c) \lor \text{Food}(c)$ & 4, 11 \\
					13. & $\text{Food}(\text{Peanuts})$ & 6, 12 \\
				\end{tabular}

				\textbf{Contradiction} between statements 10 and 13. Therefore John likes peanuts.

			\item Use resolution to answer the question "What food does Sue eat?"

				\begin{tabular}{ l l r }
					1. & $\neg \text{Food}(a) \lor \text{Likes}(\text{John}, a)$ & \\
					2. & $\text{Food}(\text{Apples})$ & \\
					3. & $\text{Food}(\text{Chicken})$ & \\
					4. & $\neg \text{Eats}(b, c) \lor  \text{\text{Kills}}(c, b) \lor \text{Food}(c)$ & \\
					5. & $\neg \text{Kills}(e, d) \lor \neg \text{Alive}(d)$ & \\
					6. & $\text{Eats}(\text{Bill}, \text{Peanuts})$ & \\
					7. & $\text{Alive}(\text{Bill})$ & \\
					8. & $\neg \text{Eats}(\text{Bill}, f) \lor \text{Eats}(\text{Sue}, f)$ & \\
					9. & $\neg \text{Eats}(\text{Sue}, \text{Peanuts})$ & \\
					\toprule
					10. & $\text{Eats}(\text{Sue}, \text{Peanuts})$ & 6, 8 \\
				\end{tabular}

				\textbf{Contradiction} between statements 10 and 13. Therefore Sue eats peanuts.

			\item Use resolution to answer (d) if, instead of the axiom marked with an asterisk above we had:

				\begin{itemize}
					\item If you don't eat you die.
					\item If you die, you are not alive.
					\item Bill is alive.
				\end{itemize}

				Converted to first-order logic:

				\begin{itemize}
					\item $\forall x \forall y (\neg \text{Eats}(x, y) \Rightarrow \text{Dies}(x))$
					\item $\forall x (\text{Dies}(x) \Rightarrow \neg \text{Alive}(x))$
					\item $\text{Alive}(\text{Bill})$
				\end{itemize}

				Converted to CNF:

				\begin{itemize}
					\item $\text{Eats}(g, h) \lor \text{Dies}(g)$
					\item $\neg \text{Dies}(i) \lor \neg \text{Alive}(i)$
					\item $\text{Alive}(\text{Bill})$
				\end{itemize}

				New knowledge base:

				\begin{tabular}{ l l r }
					1. & $\neg \text{Food}(a) \lor \text{Likes}(\text{John}, a)$ & \\
					2. & $\text{Food}(\text{Apples})$ & \\
					3. & $\text{Food}(\text{Chicken})$ & \\
					4. & $\neg \text{Eats}(b, c) \lor  \text{\text{Kills}}(c, b) \lor \text{Food}(c)$ & \\
					5. & $\neg \text{Kills}(e, d) \lor \neg \text{Alive}(d)$ & \\
					8. & $\neg \text{Eats}(\text{Bill}, f) \lor \text{Eats}(\text{Sue}, f)$ & \\
					9. & $\text{Eats}(g, h) \lor \text{Dies}(g)$ & \\
					10. & $\neg \text{Dies}(i) \lor \neg \text{Alive}(i)$ & \\
					11. & $\text{Alive}(\text{Bill})$ & \\				
					12. & $\neg \text{Eats}(\text{Sue}, \text{Apples})$ & \\
					\toprule
					13. & $\text{Dies}(\text{Sue})$ & 9, 12 \\
					14. & $\neg \text{Alive}(\text{Sue})$ & 10, 13 \\
					15. & $\neg \text{Kills}(e, \text{Bill})$ & 5, 11 \\
					16. & $\neg \text{Eats}(\text{Bill}, \text{Apples})$ & 8, 12 \\
					17. & $\text{Dies}(\text{Bill})$ & 9, 16 \\
					18. & $\neg \text{Alive}(\text{Bill})$ & 10, 17 \\
				\end{tabular}

				\textbf{Contradiction} between statements 11 and 18. Therefore Sue eats apples.
		\end{enumerate}
\end{enumerate}

\end{document}